Update

phoas.v
@@ -1,4 +1,4 @@
-Definition name := nat.
+(* Definition name := nat.
 
 Inductive term : Set := 
   | term_var : name -> term
@@ -16,16 +16,16 @@ Inductive type : Set :=
   | type_var : name -> type
   | type_arrow : type -> type -> type.
 
-Fixpoint subst (x : name) (new : term) (t : term) : term :=
+Fixpoint flatten (x : name) (new : term) (t : term) : term :=
   match t with
   | term_var y => if Nat.eqb x y then new else t
-  | term_app t1 t2 => term_app (subst x new t1) (subst x new t2)
-  | term_abs f => term_abs (fun y => if Nat.eqb x y then f y else subst x new (f y))
+  | term_app t1 t2 => term_app (flatten x new t1) (flatten x new t2)
+  | term_abs f => term_abs (fun y => if Nat.eqb x y then f y else flatten x new (f y))
   end.
 
 Inductive step : term -> term -> Prop :=
   | step_beta : forall f g x,
-      step (term_app (term_abs f) g) (subst x g (f x))
+      step (term_app (term_abs f) g) (flatten x g (f x))
   | step_app1 : forall t1 t1' t2,
       step t1 t1' ->
       step (term_app t1 t2) (term_app t1' t2)
@@ -34,4 +34,94 @@ Inductive step : term -> term -> Prop :=
       step (term_app t1 t2) (term_app t1 t2')
   | step_abs : forall f f',
       (forall x, step (f x) (f' x)) ->
-      step (term_abs f) (term_abs f').
+      step (term_abs f) (term_abs f'). *)
+
+From Stdlib Require Import Program.Equality.
+
+Definition name := nat.
+
+Inductive type : Type :=
+  | type_var : name -> type
+  | type_fun : type -> type -> type.
+
+Hint Constructors type.
+Infix "-->" := type_fun (right associativity, at level 60).
+
+Inductive term' {var : type -> Type} : type -> Type :=
+  | term_var' : forall {ty}, var ty -> term' ty
+  | term_app' : forall {arg} {res}, term' (arg --> res) -> term' arg -> term' res
+  | term_abs' : forall {arg} {res}, (var arg -> term' res) -> term' (arg --> res).
+
+Hint Constructors term'.
+Infix "@" := term_app' (left associativity, at level 50).
+
+Definition term ty := forall var, term' (var := var) ty.
+Definition term1 (ty_free : type) (ty : type) := 
+  forall var, var ty_free -> term' (var := var) ty. 
+Definition term_app {arg} {res} (f : term (arg --> res)) (arg : term arg) : term res :=
+  fun var => term_app' (f var) (arg var).
+Definition term_abs {arg} {res} (t : term1 arg res) : term (arg --> res) :=
+  fun var => term_abs' (fun x => t var x).
+
+Fixpoint flatten {var : type -> Type} {ty : type} (t : term' (var := term') ty) {struct t} : term' ty :=
+  match t with
+  | term_var' v => v
+  | term_app' f arg => term_app' (flatten f) (flatten arg)
+  | term_abs' f => term_abs' (fun x => flatten (f (term_var' (var := var) x)))
+  end.
+
+Definition subst {ty1} {ty2} (inner : term ty1) (outer : term1 ty1 ty2) : term ty2 := 
+  fun var => flatten (outer (term' (var := var)) (inner var)).
+
+Inductive is_value : forall {ty}, term ty -> Prop :=
+  | is_value_abs : forall {arg} {res} (f : term1 arg res), is_value (term_abs f).
+
+Hint Constructors is_value.
+
+Reserved Notation "t ==> t'" (no associativity, at level 90).
+Inductive step : forall {ty}, term ty -> term ty -> Prop :=
+  | step_beta :
+      forall arg res (f : term1 arg res) (v : term arg),
+      is_value v ->
+      term_app (term_abs f) v ==> subst v f
+  | step_app1 :
+      forall {arg} {res} {t1 : term (arg --> res)} {t1' : term (arg --> res)} {t2 : term arg},
+      t1 ==> t1' ->
+      step (ty := res) (term_app t1 t2) (term_app t1' t2)
+  | step_app2 :
+      forall {arg} {res} {t1 : term (arg --> res)} {t2 : term arg} {t2' : term arg},
+      t2 ==> t2' ->
+      step (ty := res) (term_app t1 t2) (term_app t1 t2')
+  where "t ==> t'" := (step t t').
+
+Hint Constructors step.
+
+Theorem preservation : forall {ty} (t t' : term ty),
+  step t t' ->
+  True.
+Proof. intros. trivial. Qed.
+
+Inductive closed_term : forall {ty}, term ty -> Prop :=
+  | closed_app : forall {arg} {res} (f : term (arg --> res)) (t : term arg),
+      closed_term f ->
+      closed_term t ->
+      closed_term (term_app f t)
+  | closed_abs : forall {arg} {res} (f : term1 arg res),
+      closed_term (term_abs f).
+
+Hint Constructors closed_term.
+
+Axiom every_term_closed : forall {ty} (t : term ty), closed_term t.
+
+Theorem progress : forall {ty} (t : term ty), 
+  closed_term t -> is_value t \/ (exists t', step t t').
+Proof. 
+  intros. 
+  induction H.
+  { destruct IHclosed_term1; auto; destruct IHclosed_term2; auto.
+    { right. inversion H1; subst. simpl_existT; subst. exists (subst t f0). eapply step_beta; auto. }
+    { right. destruct H2 as [t' Ht']. exists (term_app f t'). eapply step_app2; auto. }
+    { right. destruct H1 as [t' Ht']. exists (term_app t' t). eapply step_app1; auto. }
+    { right. destruct H1 as [f' Hf']. exists (term_app f' t). eapply step_app1; auto. } }
+  { left. constructor. }
+Qed.
